lam_kes_cbn.v
@@ -1,0 +1,731 @@
+Require Import Util.
+Require Import refocusing_lang.
+Require Import reduction_semantics_props.
+
+
+
+Inductive pnat : Set := POne | PS : pnat -> pnat.
+Fixpoint pnat2nat n := match n with POne => 1 | PS n => S (pnat2nat n) end.
+Coercion pnat2nat : pnat >-> nat.
+
+Lemma pnat2nat_injective : forall m n, pnat2nat m = pnat2nat n -> m = n.
+Proof.
+  induction m; 
+      intros n H; 
+      destruct n; inversion H; subst.
+  - auto.
+  - destruct n; discriminate.
+  - destruct m; discriminate.
+  - f_equal; auto.
+Qed.
+
+
+
+Inductive plist (T : Set) : Set := 
+| PSingle : T -> plist T
+| PCons   : T -> plist T -> plist T.
+Arguments PSingle {T} _. Arguments PCons {T} _ _.
+
+Fixpoint plist2list {T} (l : plist T) :=
+    match l with
+    | PSingle e => (e::nil) %list
+    | PCons e l => (e::plist2list l) %list
+    end.
+Coercion plist2list : plist >-> list.
+
+Fixpoint pcons2 {T : Set} (e : T) (l : list T) := 
+    match l with nil => PSingle e | cons e' l => PCons e (pcons2 e' l) end.
+
+
+Lemma plist2list_injective : forall {T} (l1 l2 : plist T), (l1 : list T) = l2 -> l1 = l2.
+Proof.
+  intro T.
+  induction l1;
+      intros l2 H;
+      destruct l2; inversion H; subst.
+  - auto.
+  - destruct l2; discriminate.
+  - destruct l1; discriminate.
+  - f_equal; auto.
+Qed.
+
+
+Lemma pcons2_injective : forall {T : Set} (e1 e2 : T) (l1 l2 : list T), 
+                             pcons2 e1 l1 = pcons2 e2 l2 -> e1 = e2 /\ l1 = l2.
+Proof.
+  intros T e1 e2 l1; revert e1 e2.
+  induction l1; intros e1 e2 l2 H;
+  destruct l2; inversion H; subst.
+  - auto.
+  - destruct (IHl1 a t l2 H2); subst; auto.
+Qed.
+
+
+Lemma pcons2_and_pcons : forall {T : Set} (e : T) (l : plist T), PCons e l = pcons2 e l.
+Proof. 
+  intros T e l; revert e.
+  induction l; intro e;
+  simpl; 
+  solve [f_equal; eauto].
+Qed.
+
+
+
+
+
+Module Lam_KES_CBN <: REF_LANG.
+
+
+  Inductive term0 : Set :=
+  | Lam0: pnat  -> term0 -> term0
+  | App0: term0 -> term0 -> term0
+  | Var0: nat   -> nat   -> term0.
+
+
+  Inductive closure : Set :=
+  | Cl : term0 -> plist (list closure) -> closure.
+
+  Notation thunk := (list closure).
+  Notation env   := (plist thunk).
+
+
+  Inductive term' : Set :=
+  | Cl_t  : closure          -> term'
+  | App   : term' -> closure -> term'.
+  Coercion Cl_t : closure >-> term'.
+  Definition term := term'.
+  Hint Unfold term.
+
+
+  Definition elem_context := closure.
+  Hint Unfold elem_context.
+
+  Definition elem_plug (t : term) (ec : elem_context) : term := App t ec.
+  Notation "ec :[ t ]" := (elem_plug t ec) (at level 0).
+
+
+  Definition ckind : Set := unit.
+  Hint Unfold ckind.
+
+  Definition ckind_trans (k : ckind) (ec : elem_context) : ckind := tt.
+  Infix "+>" := ckind_trans (at level 50, left associativity).
+
+
+  Inductive context (k1 : ckind) : ckind -> Set :=
+  | empty : context k1 k1
+  | ccons : forall (ec : elem_context) {k2}, context k1 k2 -> context k1 (k2+>ec).
+  Arguments empty {k1}. Arguments ccons {k1} _ {k2} _.
+
+  Notation "[.]"      := empty.
+  Notation "[.]( k )" := (@empty k).
+  Infix    "=:"       := ccons (at level 60, right associativity).
+
+
+  Fixpoint compose {k1 k2} (c0 : context k1 k2) 
+                      {k3} (c1 : context k3 k1) : context k3 k2 := 
+      match c0 in context _ k2' return context k3 k2' with
+      | [.]     => c1
+      | ec=:c0' => ec =: compose c0' c1
+      end.
+  Infix "~+" := compose (at level 60, right associativity).
+
+
+  Fixpoint plug (t : term) {k1 k2} (c : context k1 k2) : term :=
+      match c with
+      | [.]    => t 
+      | ec=:c' => plug ec:[t] c'
+      end.
+  Notation "c [ t ]" := (plug t c) (at level 0).
+
+
+  Definition immediate_ec ec t := exists t', ec:[t'] = t.
+
+
+  Inductive value' : Set := 
+  | vLam_cl : pnat -> term0 -> env -> value'.
+  Definition value (_: ckind) := value'.
+
+  Definition value_to_term {k} (v : value k) : term :=
+      match v with vLam_cl n t e => Cl (Lam0 n t) e end.
+  Coercion  value_to_term : value >-> term.
+
+
+  Inductive redex' : Set :=
+  | rBeta   : pnat -> term0 -> thunk -> list thunk -> closure -> redex'
+  | rSubApp : term0 -> term0 -> env -> redex'
+  | rSubVar : nat -> nat -> env -> redex'.
+  Definition redex (_: ckind) := redex'.
+
+  Definition redex_to_term {k} (r : redex k) : term :=
+      match r with 
+      | rBeta n t th e cl  => App (Cl (Lam0 n t) (pcons2 th e)) cl 
+      | rSubApp t1 t2 e => Cl (App0 t1 t2) e
+      | rSubVar p o e   => Cl (Var0 p o) e
+      end.
+  Coercion  redex_to_term : redex >-> term.
+
+
+  Definition init_ckind : ckind     := tt.
+  Definition dead_ckind (_ : ckind) := False.
+
+
+  Definition contract {k} (r : redex k) : option term :=
+      match r with
+      | rBeta POne   t th e cl => Some (Cl t (PCons nil (pcons2 (cl::th)%list e)) : term)
+      | rBeta (PS n) t th e cl => Some (Cl (Lam0 n t) (pcons2 (cl::th)%list e) : term)
+      | rSubApp t1 t2 e => Some (App (Cl t1 e) (Cl t2 e))
+      | rSubVar p o e => match List.nth_error e p with 
+                         | None => None
+                         | Some th => option_map Cl_t (List.nth_error th o)
+                         end
+      end.
+
+
+  Inductive decomp k : Set :=
+  | d_red : forall {k'}, redex k' -> context k k' -> decomp k
+  | d_val : value k -> decomp k.
+  Arguments d_val {k} _. Arguments d_red {k} {k'} _ _.
+
+  Definition decomp_to_term {k} (d : decomp k) :=
+      match d with
+      | d_val v     => value_to_term v
+      | d_red _ r c => c[r]
+      end.
+  Coercion decomp_to_term : decomp >-> term.
+
+
+  Definition immediate_subterm t0 t := exists ec, t = ec:[t0].
+
+  Definition subterm_order := clos_trans_1n term immediate_subterm.
+  Notation "t1 <| t2" := (subterm_order t1 t2) (at level 70, no associativity).
+
+
+
+
+  Lemma elem_plug_injective1 : 
+      forall ec {t0 t1}, ec:[t0] = ec:[t1] -> t0 = t1.
+
+  Proof. 
+    intros ec t0 t1 H.
+    destruct ec; inversion H; 
+    auto.
+  Qed.
+
+
+  Lemma value_to_term_injective : 
+      forall {k} (v v' : value k), value_to_term v = value_to_term v' -> v = v'.
+
+  Proof.
+    intros k v v' H.
+    destruct v, v'; inversion H; subst.
+    f_equal.
+  Qed.
+
+
+  Lemma redex_to_term_injective : 
+      forall {k} (r r' : redex k), redex_to_term r = redex_to_term r' -> r = r'.
+
+  Proof.
+    intros k r r' H.
+    destruct r, r'; inversion H; subst; 
+    try solve [ f_equal;
+                eauto using plist2list_injective ].
+    - destruct (pcons2_injective _ _ _ _ H3); subst; auto.
+  Qed.
+
+
+  Lemma death_propagation : 
+      forall k, dead_ckind k -> forall ec, dead_ckind (k+>ec).
+
+  Proof. auto. Qed.
+
+  Lemma proper_death : 
+      forall k, dead_ckind k -> ~ exists (r : redex k), True.
+
+  Proof. auto. Qed.
+
+
+  Lemma value_trivial1 : forall {k} (v : value k) ec {t}, 
+                             ~dead_ckind (k+>ec) -> ec:[t] = v -> 
+                                 exists (v' : value (k+>ec)), t = v'.
+
+  Proof. intros k v ec t H H0. destruct ec, v; discriminate. Qed.
+
+
+  Lemma value_redex    : forall {k} (v : value k) (r : redex k), 
+                             value_to_term v <> redex_to_term r.
+  Proof. intros k v r. destruct v, r; eauto. Qed.
+
+
+  Lemma redex_trivial1 : forall {k} (r : redex k) ec t, 
+                             ~dead_ckind (k+>ec) -> ec:[t] = r -> 
+                                 exists (v : value (k+>ec)), t = v.
+  Proof. 
+    intros k r ec t H H0. 
+    destruct ec, r; inversion H0; subst.
+    - eexists (vLam_cl _ _ _); reflexivity.
+  Qed.
+
+
+  Lemma wf_immediate_subterm : well_founded immediate_subterm.
+  Proof. REF_LANG_Help.prove_st_wf. Qed.
+
+
+  Definition wf_subterm_order : well_founded subterm_order
+      := wf_clos_trans_l _ _ wf_immediate_subterm.
+
+
+
+  (* Extras *)
+  Fixpoint closed_within (t : term0) (el : plist nat) : Prop :=
+      match t with
+      | Lam0 n t   => match el with 
+                      | PSingle m  => closed_within t (PCons 0 (PSingle(n + m)))
+                      | PCons m el => closed_within t (PCons 0 (PCons (n + m) el))
+                      end
+      | App0 t1 t2 => closed_within t1 el /\ closed_within t2 el
+      | Var0 p o   => match List.nth_error el p with
+                      | None   => False
+                      | Some n => o < n
+                      end
+      end.
+
+
+  Fixpoint env_layout (e : env) : plist nat := 
+      match e with
+      | PSingle th => PSingle (List.length th)
+      | PCons th e => PCons (List.length th) (env_layout e)
+      end.
+
+
+  Inductive closed_cl : closure -> Prop :=
+  | cc : forall t (e : env), closed_within t (env_layout e) -> closed_env e -> 
+                                 closed_cl (Cl t e)
+
+  with closed_env : env -> Prop :=
+  | ce1 : forall th, closed_th th                   -> closed_env (PSingle th)
+  | ce2 : forall th e, closed_th th -> closed_env e -> closed_env (PCons th e)
+
+  with closed_th : thunk -> Prop :=
+  | ct1 : closed_th nil
+  | ct2 : forall cl th, closed_cl cl -> closed_th th -> closed_th (cl :: th)%list.
+
+  Scheme cc_Ind := Induction for closed_cl  Sort Prop
+    with ce_Ind := Induction for closed_env Sort Prop
+    with ct_Ind := Induction for closed_th  Sort Prop.
+
+
+  Fixpoint closed (t : term) : Prop := 
+      match t with 
+      | Cl_t cl  => closed_cl cl
+      | App t cl => closed t /\ closed_cl cl
+      end.
+
+
+  Lemma env_thunks_closed : 
+      forall e n th, closed_env e -> List.nth_error e n = Some th -> closed_th th.
+
+  Proof.
+    intros e n th H; revert n th.
+    induction H; intros n th' H1.
+    - destruct n as [ | [ | ?]];
+      simpl in H1; unfold Specif.value in H1; inversion H1; subst; auto.
+    - destruct n as [ | n].
+      + simpl in H1; unfold Specif.value in H1; inversion H1; subst; auto.
+      + simpl in H1; eauto.
+  Qed.
+
+
+  Lemma thunk_closures_closed :
+      forall th n cl, closed_th th -> List.nth_error th n = Some cl -> closed_cl cl.
+  Proof.
+    intros th n cl H; revert n cl.
+    induction H; 
+        intros n cl' H1;
+        destruct n;
+        inversion H1; subst;
+    solve [eauto].
+  Qed.
+
+
+  Lemma env_layout_nth_is_th_size : 
+      forall (e : env) n th m, 
+          List.nth_error e n = Some th -> List.nth_error (env_layout e) n = Some m -> 
+              m = List.length th.
+  Proof.
+    intros e n; revert e.
+    induction n as [ | n];
+        intros e th m H H0;
+        destruct e as [th1 | th1 e]; inversion H; subst;
+    solve 
+    [ inversion H0;
+      auto
+    | destruct n; discriminate
+    | eauto ].
+  Qed. 
+
+
+  Lemma env_layout_semi_correct : 
+      forall (e : env) n, List.nth_error e n = None <-> 
+                              List.nth_error (env_layout e) n = None.
+  Proof.
+    intros e n; revert e.
+    induction n as [ | n]; 
+        intros e; split; intro H;
+        destruct e; inversion H; subst; 
+    solve
+    [ auto
+    | destruct n; auto
+    | apply IHn; auto ].
+  Qed. 
+
+
+  Require Import Arith.
+
+  Lemma nth_error_safe : forall {T} (l : list T) n, n < List.length l -> 
+                             exists e, List.nth_error l n = Some e.
+  Proof.
+    intros T l n; revert l.
+    induction n; intros l H.
+    - destruct l.
+      + contradict H; auto with arith.
+      + exists t; auto.
+    - destruct l.
+      + contradict H; auto with arith.
+      + assert (n < length l).
+        { auto with arith. }
+        eauto.
+  Qed.
+
+
+
+  Lemma contract_closed : forall {k} (r : redex k), 
+                              closed r -> exists t, contract r = Some t /\ closed t.
+
+  Let Ar : forall m n, S (m + n) = m + S n. 
+  Proof. auto with arith. Qed.
+
+  Proof.
+    intros k r H.
+    destruct r; simpl in H.
+
+    - destruct p as [ | n];
+      [ exists (Cl t (PCons nil (pcons2 (c::l)%list l0)))
+      | exists (Cl (Lam0 n t) (pcons2 (c::l)%list l0))];
+      simpl; intuition;
+          inversion H0; subst;
+          destruct l0; simpl in H3;
+          try rewrite Ar in H3;
+          inversion H4; subst;
+      solve [repeat (constructor; auto)].
+
+    - eexists. intuition. 
+      inversion H; subst.
+      simpl in *.
+      split; 
+      solve [constructor; intuition].
+
+    - inversion H; subst.
+      cut (exists th, List.nth_error p n = Some th /\ 
+           exists cl, List.nth_error th n0 = Some cl).
+      {
+          intros [th [H0 [cl H1]]].
+          exists cl.
+          simpl.
+          rewrite H0.
+          rewrite H1.
+          eauto using thunk_closures_closed, env_thunks_closed.
+      }
+
+      simpl in H2.
+      remember (List.nth_error (env_layout p) n) as th_size_o; 
+      destruct th_size_o as [n1 | ]; autof.
+      remember (List.nth_error p n) as th_o; 
+      destruct th_o as [th | ];
+          symmetry in Heqth_size_o, Heqth_o.
+      + assert (n1 = length th). 
+        { eauto using env_layout_nth_is_th_size. }
+        exists th.
+        intuition.
+        subst.
+        destruct (nth_error_safe th n0) as [cl H1]; auto.
+        solve [eauto].
+      + apply env_layout_semi_correct in Heqth_o.
+        congruence.
+  Qed.
+
+
+  Lemma context_closed : forall {k1 k2} (c : context k1 k2) t, closed c[t] -> closed t.
+  Proof.
+    induction c; intros t H.
+    - auto.
+    - assert (closed ec:[t]); auto.
+      destruct ec; inversion H0; subst.
+      auto.
+  Qed.
+
+
+  Lemma plug_replace_closed : forall {k1 k2} (c : context k1 k2) t1 t2, 
+                                  closed c[t1] -> closed t2 -> closed c[t2].
+  Proof.
+    induction c; intros t1 t2 H H0.
+    - auto.
+    - apply (IHc ec:[t1]); auto. 
+      simpl in H.
+      apply context_closed in H; simpl in H.
+      simpl.
+      intuition.
+  Qed.
+
+
+  Lemma red_step_closed : 
+      forall {k1 k2} (c : context k1 k2) (r : redex k2), closed c[r] -> 
+          exists t, contract r = Some t /\ closed c[t].
+  Proof.
+    intros ? ? ? r ?.
+    destruct (contract_closed r) as [t [H0 H1]].
+    { eauto using context_closed. }
+    exists t.
+    eauto using plug_replace_closed.
+  Qed.
+
+End Lam_KES_CBN.
+
+
+
+
+Module Lam_KES_CBN_Strategy <: REF_STRATEGY Lam_KES_CBN.
+
+  Import Lam_KES_CBN.
+
+
+  Inductive interm_dec k : Set :=
+  | in_red  : redex k -> interm_dec k
+  | in_term : term -> elem_context -> interm_dec k
+  | in_val  : value k -> interm_dec k
+  | in_dead : interm_dec k.
+  Arguments in_red {k} _.    Arguments in_val {k} _.
+  Arguments in_term {k} _ _. Arguments in_dead {k}.
+
+
+  Definition dec_term (t : term) (k : ckind) : interm_dec k :=
+      match t with
+      | Cl_t (Cl (Lam0 n t) e)   => in_val (vLam_cl n t e)
+      | Cl_t (Cl (App0 t1 t2) e) => in_red (rSubApp t1 t2 e)
+      | Cl_t (Cl (Var0 p o) e)   => in_red (rSubVar p o e)
+      | App t cl                 => in_term t cl
+      end.
+
+
+  Definition dec_context (ec : elem_context) (k : ckind) (v : value (k+>ec)) 
+                 : interm_dec k :=
+      match v with
+      | vLam_cl n t e => match e with PSingle th => in_red (rBeta n t th nil ec)
+                                    | PCons th e => in_red (rBeta n t th e ec)
+                                 end
+      end.
+
+
+  Lemma dec_term_correct : 
+      forall t k, match dec_term t k with
+      | in_red r      => t = r
+      | in_val v      => t = v
+      | in_term t' ec => t = ec:[t']
+      | in_dead       => dead_ckind k
+      end.
+  Proof.
+    destruct t,k; simpl.
+    - destruct c; destruct t; auto.
+    - auto.
+  Qed.
+
+
+  Lemma dec_term_from_dead : forall t k, 
+      dead_ckind k -> dec_term t k = in_dead.
+  Proof. inversion 1. Qed.
+
+
+  Lemma dec_context_correct : 
+      forall ec k v, match dec_context ec k v with
+      | in_red r      => ec:[v] = r
+      | in_val v'     => ec:[v] = v'
+      | in_term t ec' => ec:[v] = ec':[t]
+      | in_dead       => dead_ckind (k+>ec) 
+      end.
+  Proof.
+    destruct ec, k, v.
+    destruct p1; simpl.
+    - auto.
+    - unfold elem_plug. 
+      repeat (f_equal; eauto using pcons2_and_pcons).
+  Qed.
+
+
+  Lemma dec_context_from_dead : forall ec k (v : value (k+>ec)), 
+      dead_ckind (k+>ec) -> dec_context ec k v = in_dead.
+  Proof. inversion 1. Qed.
+
+
+  Lemma dec_term_next_alive : forall t k {t0 ec0}, 
+      dec_term t k = in_term t0 ec0 -> ~ dead_ckind (k+>ec0).
+  Proof. auto. Qed.
+
+
+  Lemma dec_context_next_alive : forall ec k v {t0 ec0}, 
+      dec_context ec k v = in_term t0 ec0 -> ~ dead_ckind (k+>ec0).
+  Proof. auto. Qed.
+
+
+  Lemma dec_context_not_val : 
+      forall ec {k} (v1 : value k) v0, 
+          dec_context ec k v0 <> in_val v1.
+  Proof.
+    intros ec k v1 v0 H.
+    destruct ec, k, v0.
+    destruct p1;
+    inversion H.
+  Qed.
+
+
+  Lemma dec_term_value : 
+      forall {k} (v : value k), dec_term v k = in_val v.
+  Proof.
+    intros k v.
+    destruct v, k.
+    auto.
+  Qed.
+
+
+
+
+  Definition search_order : ckind -> term -> elem_context -> elem_context -> Prop := 
+      fun _ _ _ _ => False.
+  Notation "k , t |~  ec1 << ec2 " := (search_order k t ec1 ec2) 
+               (at level 70, t, ec1, ec2 at level 50, no associativity).
+
+
+  Lemma dec_term_term_top : 
+      forall t k {t' ec}, dec_term t k = in_term t' ec -> 
+          forall ec',  ~ k, t |~ ec << ec'.
+  Proof. auto. Qed.
+
+
+  Lemma dec_context_red_bot : 
+      forall k ec v {r : redex k}, dec_context ec k v = in_red r -> 
+          forall ec',  ~ k, ec:[v] |~ ec' << ec.
+  Proof. auto. Qed.
+
+
+  Lemma dec_context_val_bot : 
+      forall k ec v {v' : value k}, dec_context ec k v = in_val v' -> 
+          forall ec',  ~ k, ec:[v] |~ ec' << ec.
+  Proof. auto. Qed.
+
+
+  Lemma dec_context_term_next : 
+      forall ec0 k v {t ec1}, dec_context ec0 k v = in_term t ec1 -> 
+      (*1*) k, ec0:[v] |~ ec1 << ec0 /\ 
+      (*2*) forall ec,  k, ec0:[v] |~ ec << ec0  ->  ~ k, ec0:[v] |~ ec1 << ec.
+  Proof.
+    intros ec k; destruct ec, k, v.
+    destruct p1;
+    inversion 1.
+  Qed.
+
+
+  Lemma elem_context_det : 
+      forall t ec {t'}, t = ec:[t'] -> 
+          forall k ec',  k, t |~ ec' << ec -> 
+              exists (v : value (k+>ec)), t' = v.
+  Proof. inversion 2. Qed.
+
+
+  Lemma wf_search : forall k t, well_founded (search_order k t).
+  Proof. intros k t ec. constructor. inversion 1. Qed.
+
+
+  Lemma search_order_antisym : forall k t ec ec0, 
+      k, t |~ ec << ec0 -> ~ k, t |~ ec0 << ec.
+  Proof. auto. Qed.
+
+
+  Lemma search_order_trans   : forall k t ec0 ec1 ec2,
+      k, t |~ ec0 << ec1 -> k, t |~ ec1 << ec2 -> k,t |~ ec0 << ec2.
+  Proof. auto. Qed.
+
+
+  Lemma search_order_comp_if : 
+      forall t ec0 ec1, immediate_ec ec0 t -> immediate_ec ec1 t -> 
+          forall k, ~ dead_ckind (k+>ec0) -> ~ dead_ckind (k+>ec1) ->
+              k, t |~ ec0 << ec1  \/  k, t |~ ec1 << ec0  \/  ec0 = ec1.
+  Proof.
+    intros t ec0 ec1 H1 H2 k H3 H4.
+    destruct H1 as [t' H1], H2 as [t'' H2].
+    destruct ec0, ec1, t; inversion H1; inversion H2; subst.
+    inversion H7; subst.
+    auto.
+  Qed.
+
+
+  Lemma search_order_comp_fi : 
+      forall k t ec0 ec1,  k, t |~ ec0 << ec1 ->  
+          immediate_ec ec0 t /\ immediate_ec ec1 t /\ 
+              ~ dead_ckind (k+>ec0) /\ ~ dead_ckind (k+>ec1).
+  Proof. inversion 1. Qed.
+
+End Lam_KES_CBN_Strategy.
+
+
+
+
+Module Lam_KES_CBN_Cal.
+  Module RefLang := Lam_KES_CBN.
+  Module RefStrategy := Lam_KES_CBN_Strategy.
+  Module RedLang := RedRefLang RefLang RefStrategy.
+End Lam_KES_CBN_Cal.
+
+
+
+
+Module Lam_KES_CBN_SafeReg <: SAFE_RED_REGION Lam_KES_CBN_Cal.RedLang.
+
+  Import Lam_KES_CBN.
+
+  Definition safe (_ : ckind) t : Prop := closed t.
+
+  Definition progresvation : 
+      forall {k1 k2} (c : context k1 k2) (r : redex k2), safe k1 c[r] -> 
+          exists t, contract r = Some t /\ safe k1 c[t] 
+
+      := @red_step_closed.
+
+End Lam_KES_CBN_SafeReg.
+
+
+
+
+Require Import refocusing_semantics_derivation.
+Require Import abstract_machine.
+Require Import refocusing_machine.
+Require Import refocusing_machine_safe_reg.
+
+
+Module Lam_KES_CBN_RefSem <: PE_RED_REF_SEM Lam_KES_CBN_Cal.RedLang.
+
+  Include RedRefSem Lam_KES_CBN_Cal.
+
+  Definition dec_context_not_val := Lam_KES_CBN_Strategy.dec_context_not_val.
+  Definition dec_term_value      := @Lam_KES_CBN_Strategy.dec_term_value.
+  Arguments  dec_term_value {k} _.
+
+End Lam_KES_CBN_RefSem.
+
+
+Module EAKrivineMachine := RefEvalApplyMachine Lam_KES_CBN_Cal.RedLang Lam_KES_CBN_RefSem.
+Module KrivinMachine    := RefPushEnterMachine Lam_KES_CBN_Cal.RedLang Lam_KES_CBN_RefSem.
+
+Module EAKrivineMachine_SafeReg <: AM_SAFE_REGION EAKrivineMachine := 
+
+    RefEAMSafeReg  Lam_KES_CBN_Cal.RedLang  Lam_KES_CBN_RefSem 
+                               EAKrivineMachine  Lam_KES_CBN_SafeReg.
+
