reduction_semantics_props.v
@@ -1,0 +1,161 @@
+Require Import reduction_semantics reduction_semantics_facts.
+
+
+Coercion bool2prop b := match b with true => True | false => False end.
+
+
+Module Type SAFE_RED_REGION (R : RED_LANG).
+
+  Import R.
+
+  Parameter safe : ckind -> term -> Prop.
+  Axiom progresvation : 
+      forall {k1 k2} (c : context k1 k2) (r : redex k2), 
+          safe k1 c[r] -> exists t, contract r = Some t /\ safe k1 c[t].
+  (*Axiom safe_decomp1  : forall k t ec t', safe k t -> t = ec:[t'] -> 
+                            ~dead_ckind (k+>ec) -> safe (k+>ec) t'.*)
+
+End SAFE_RED_REGION.
+
+
+
+(*
+Module SAFE_RED_REGION_Facts (R : RED_LANG) (Reg : SAFE_RED_REGION R).
+
+  Module RF := RED_LANG_Facts R.
+  Import R Reg RF.
+
+  Lemma safe_decomp : forall {k1 k2} (c : context k1 k2) t, ~dead_ckind k2 -> 
+                          safe k1 c[t] -> safe k2 t.
+  Proof.
+    intros k1 k2 c.
+    induction c; intros t H H0;
+    solve [eauto using safe_decomp1, death_propagation2].
+  Qed.
+
+End SAFE_RED_REGION_Facts.
+  *)  
+
+
+(*
+Module Type INIT_RED_SAFE (R : RED_LANG) (Reg : SAFE_RED_REGION R).
+
+  Import R Reg.
+  Axiom init_safe : forall t, safe init_ckind t.
+
+End INIT_RED_SAFE.*)
+
+
+(*
+Module Type RED_CAL.
+  Declare Module RedLang : RED_LANG.
+  Declare Module RedSem  : RED_SEM RedLang.
+End RED_CAL.
+
+
+
+Module SAFE_SUB_REF (R : RED_LANG) (S : RED_SEM R) (Reg : SAFE_RED_REGION R) 
+                        (*IS : INIT_RED_SAFE R Reg*) <: RED_CAL.
+
+  Module Type CS.
+    Inductive context (k1 : R.ckind) : R.ckind -> Set :=
+    | empty : context k1 k1
+    | ccons : forall (ec : R.elem_context) {k2}, context k1 k2 -> context k1 (R.ckind_trans k2 ec).
+    Arguments empty {k1}. Arguments ccons {k1} _ {k2} _.
+    
+    Inductive decomp k : Set :=
+    | d_red : forall {k'}, R.redex k' -> context k k' -> decomp k
+    | d_val : R.value k -> decomp k.
+    Arguments d_red {k k'} _ _. Arguments d_val {k} _.
+    
+  End CS.
+
+  Module CSM : CS := R.
+
+  Module RedLang.
+
+    Definition term := { t | exists k, Reg.safe k t }.
+    Coercion org_term (t : term) := proj1_sig t.
+
+    Definition elem_context := R.elem_context.
+    Definition ckind := R.ckind.
+    Definition ckind_trans := R.ckind_trans.
+    Infix "+>" := ckind_trans (at level 50, left associativity).
+
+    Include CSM.
+
+    Notation "[.]"      := empty.
+    Notation "[.]( k )" := (@empty k).
+    Infix    "=:"       := ccons (at level 60, right associativity).
+
+    Fixpoint compose {k1 k2} (c0 : context k1 k2) 
+                        {k3} (c1 : context k3 k1) : context k3 k2 := 
+        match c0 in context _ k2' return context k3 k2' with
+        | [.]     => c1
+        | ec =: c0' => ec =: compose c0' c1
+        end.
+    Infix "~+" := compose (at level 60, right associativity).
+
+    Definition elem_plug (t : term) (ec : elem_context) : term. (* := *) refine (
+        exist _ (R.elem_plug t ec) _).
+    Proof. destruct t as [t [k H]]. exists (k+>ec). simpl.  eapply Reg.safe_decomp; simpl; auto.
+    
+    Notation "ec :[ t ]" := (elem_plug t ec) (at level 0).
+
+    Fixpoint plug (t : term) {k1 k2} (c : context k1 k2) : term :=
+        match c with
+        | [.]    => t 
+        | ec=:c' => plug ec:[t] c'
+        end.
+    Notation "c [ t ]" := (plug t c) (at level 0).
+
+    Axiom elem_plug_injective1 : forall ec {t0 t1}, ec:[t0] = ec:[t1] -> t0 = t1.
+
+    Definition immediate_ec ec t := exists t', ec:[t'] = t.
+
+    Parameters value redex : ckind -> Set.
+
+    Parameter value_to_term : forall {k}, value k -> term.
+    Coercion  value_to_term : value >-> term.
+    Parameter redex_to_term : forall {k}, redex k -> term.
+    Coercion  redex_to_term : redex >-> term.
+
+    Axiom value_to_term_injective : 
+        forall {k} (v v' : value k), value_to_term v = value_to_term v' -> v = v'.
+    Axiom redex_to_term_injective : 
+        forall {k} (r r' : redex k), redex_to_term r = redex_to_term r' -> r = r'.
+
+
+
+    Parameter  init_ckind : ckind.
+    Parameter  dead_ckind : ckind -> Prop. 
+
+    Axiom death_propagation : 
+        forall k, dead_ckind k -> forall ec, dead_ckind (k+>ec).
+    Axiom proper_death : 
+        forall k, dead_ckind k -> ~ exists (r : redex k), True.
+
+
+    Axiom value_trivial1 : forall {k} (v : value k) ec {t}, 
+                               ~dead_ckind (k+>ec) -> ec:[t] = v -> 
+                                   exists (v' : value (k+>ec)), t = v'.
+    Axiom value_redex    : forall {k} (v : value k) (r : redex k), 
+                               value_to_term v <> redex_to_term r.
+
+    Axiom decompose : forall (t : term) k1, ~ dead_ckind k1 ->
+        (exists (v : value k1), t = v) \/
+        (exists k2 (r : redex k2) (c : context k1 k2), t = c[r]).
+
+
+    Parameter contract : forall {k}, redex k -> option term.
+*)
+
+
+
+
+Module Type RED_PROGRESS (R : RED_LANG).
+
+  Import R.
+  Axiom progress : forall {k} (r : redex k), exists t, contract r = Some t.
+
+End RED_PROGRESS.
