refocusing_semantics.v
@@ -14,19 +14,19 @@ Module Type RED_REF_SEM (R : RED_LANG) <: RED_SEM R.
 
 
 
-  Inductive dec__ : term -> forall {k1 k2}, context k1 k2 -> decomp k1 -> Prop :=
+  Inductive dec' : term -> forall {k1 k2}, context k1 k2 -> decomp k1 -> Prop :=
 
   | d_dec  : forall t {k1 k2} (c : context k1 k2) {r},
                dec_term t k2 = in_red r -> 
-               dec__ t c (d_red r c)
+               dec' t c (d_red r c)
   | d_v    : forall t {k1 k2} {c : context k1 k2} {v d},
                dec_term t k2 = in_val v ->
                decctx v c d ->
-               dec__ t c d
+               dec' t c d
   | d_term : forall t {t0 k1 k2} {c : context k1 k2} {ec d},
                dec_term t k2 = in_term t0 ec ->
-               dec__ t0 (ec=:c) d ->
-               dec__ t c d
+               dec' t0 (ec=:c) d ->
+               dec' t c d
 
   with decctx : forall {k2}, value k2 -> 
                     forall {k1}, context k1 k2 -> decomp k1 -> Prop :=
@@ -45,14 +45,14 @@ Module Type RED_REF_SEM (R : RED_LANG) <: RED_SEM R.
   | dc_term : forall ec {ec0 k2} (v : value (k2+>ec)) 
                             {k1} {c : context k1 k2} {t d},
                 dec_context ec k2 v = in_term t ec0 ->
-                dec__ t (ec0=:c) d ->
+                dec' t (ec0=:c) d ->
                 decctx v (ec=:c) d.
 
-  Scheme dec_Ind    := Induction for dec__ Sort Prop
+  Scheme dec_Ind    := Induction for dec' Sort Prop
     with decctx_Ind := Induction for decctx Sort Prop.
 
 
-  Include RED_SEM R with Definition dec := dec__.
+  Include RED_SEM R with Definition dec := dec'.
 
 
   Axiom dec_val_self : forall {k2} (v : value k2) {k1} {c : context k1 k2} {d}, 
@@ -71,7 +71,8 @@ Module Type PE_RED_REF_SEM (R : RED_LANG) <: RED_REF_SEM R.
   Import R.
 
   Axiom dec_context_not_val : 
-      forall ec {k} v1 (v0 : value (k+>ec)), dec_context ec k v0 <> in_val v1.
+      forall ec {k} (v1 : value k) v0, 
+          dec_context ec k v0 <> in_val v1.
 
   Axiom dec_term_value : 
       forall {k} (v : value k), dec_term v k = in_val v.
